pulse/share/steel/examples/pulse/dice/lib/PulseHashTable.fst
@@ -12,48 +12,55 @@ module U8 = FStar.UInt8
 module LK = Steel.ST.SpinLock
 module PHT = LinearScanHashTable
 open LinearScanHashTable
+open Pulse.Class.BoundedIntegers
+
+type bound_us = n:US.t{US.fits (US.v n)}
+type pos_us = n:bound_us{US.v n > 0}
 
 noeq
 type ht (s : pht_sig) = {
-  sz : pos;
-  contents : A.larray (cell s.keyt s.valt) sz;
+  sz : pos_us;
+  contents : A.larray (cell s.keyt s.valt) (US.v sz);
 }
 
-let models (s:pht_sig) (pht:pht s) (ht:ht s) : vprop
+let canonical_index_us #s (k : s.keyt) (sz : pos_us) 
+  : n:US.t{US.v n == PHT.canonical_index k (US.v sz)} 
+  = US.uint_to_t (s.hashf k % US.v sz)
+
+let modulo_us (m:pos_us) (v1 v2:US.t)
+  : n:US.t{n<m}
+  = US.uint_to_t ((US.v v1 + US.v v2) % US.v m)
+
+let models (s:pht_sig) (ht:ht s) (pht:pht s) : vprop
 = A.pts_to ht.contents full_perm pht.repr `star`
-  pure (pht.sz == ht.sz)
-
-
-let coerce_nat (n:int{n>=0}) : nat = n
+  pure (pht.sz == US.v ht.sz)
 
 ```pulse
 fn pulse_lookup_index (#s:pht_sig) (#pht:(p:pht s{not_full p.repr}))  
                 (ht:ht s) (k:s.keyt)
-  requires models s pht ht
-  returns  o:(o:option (s.valt & nat){o == PHT.lookup_index pht k})
-  ensures  models s pht ht
+  requires models s ht pht
+  returns  o:(o:option (s.valt & bound_us){o == PHT.lookup_index_us pht k})
+  ensures  models s ht pht
 {
   let sz = ht.sz;
-  let cidx = canonical_index k sz;
-  let mut off = coerce_nat 0;
+  let cidx = canonical_index_us k sz;
+  let mut off = 0sz;
   let mut cont = true;
-  let mut ret = None #(s.valt & nat);
+  let mut ret = None #(s.valt & bound_us);
 
-  unfold (models s pht ht);
+  unfold (models s ht pht);
 
   while (let voff = !off; let vcont = !cont; (voff <= sz && vcont = true)) 
-  invariant b. exists (voff:nat) (vcont:bool). (
+  invariant b. exists (voff:US.t) (vcont:bool). (
     A.pts_to ht.contents full_perm pht.repr **
     R.pts_to off full_perm voff **
     R.pts_to cont full_perm vcont **
     `@(if vcont 
       then R.pts_to ret full_perm None
-      else R.pts_to ret full_perm (PHT.lookup_index pht k)) ** 
+      else R.pts_to ret full_perm (PHT.lookup_index_us pht k)) ** 
     pure (
-      pht.sz == sz /\
-      sz > 0 /\
-      voff >= 0 /\ voff <= sz /\
-      walk_get_idx pht.repr cidx k voff == lookup_repr_index pht.repr k /\
+      voff <= sz /\
+      walk_get_idx pht.repr (US.v cidx) k (US.v voff) == lookup_repr_index pht.repr k /\
       b == (voff <= sz && vcont = true)
     ))
   {
@@ -61,40 +68,35 @@ fn pulse_lookup_index (#s:pht_sig) (#pht:(p:pht s{not_full p.repr}))
     if (voff = sz) {
       cont := false;
       assert_ (R.pts_to ret full_perm None);
-      assert_ (pure (walk_get_idx pht.repr cidx k voff == None));
-      ()
+      assert_ (pure (walk_get_idx pht.repr (US.v cidx) k (US.v voff) == None));
     } else {
-      let idx = (cidx+voff)%sz;
-      let c = op_Array_Index_nat ht.contents #full_perm #pht.repr idx;
+      let idx = modulo_us sz cidx voff;
+      let c = op_Array_Index_nat ht.contents #full_perm #pht.repr (US.v idx);
       match c {
-        Used k' v' -> { 
+        Used k' v' -> {
           if (k' = k) {
             cont := false;
             write ret (Some (v',idx)) #None;
-            assert_ (pure (pht.repr @@ idx == Used k' v'));
-            assert_ (pure (lookup_repr_index pht.repr k == Some (v', idx)));
-            ()
+            assert_ (pure (pht.repr @@ US.v idx == Used k' v'));
+            assert_ (pure (lookup_repr_index pht.repr k == Some (v', US.v idx)));
           } else {
-            off := voff + 1;
-            assert_ (pure (walk_get_idx pht.repr cidx k voff == walk_get_idx pht.repr cidx k (voff+1)));
-            ()
+            off := voff + 1sz;
+            assert_ (pure (walk_get_idx pht.repr (US.v cidx) k (US.v voff) == walk_get_idx pht.repr (US.v cidx) k (US.v (voff+1sz))));
           }}
         Clean -> {
           cont := false;
-          assert_ (pure (walk_get_idx pht.repr cidx k voff == None));
-          assert_ (R.pts_to ret full_perm (lookup_repr_index #s #pht.sz pht.repr k));
-          ()
+          assert_ (pure (walk_get_idx pht.repr (US.v cidx) k (US.v voff) == None));
+          assert_ (R.pts_to ret full_perm (PHT.lookup_index_us pht k));
          }
         Zombie -> {
-          off := voff + 1;
-          assert_ (pure (walk_get_idx pht.repr cidx k voff == walk_get_idx pht.repr cidx k (voff+1)));
-          ()
+          off := voff + 1sz;
+          assert_ (pure (walk_get_idx pht.repr (US.v cidx) k (US.v voff) == walk_get_idx pht.repr (US.v cidx) k (US.v (voff+1sz))));
          }
       };
     };
   };
-  fold (models s pht ht);
-  assert_ (R.pts_to ret full_perm (lookup_repr_index #s #pht.sz pht.repr k));
+  fold (models s ht pht);
+  assert_ (R.pts_to ret full_perm (PHT.lookup_index_us pht k));
   let o = !ret;
   o
 }
@@ -103,9 +105,9 @@ fn pulse_lookup_index (#s:pht_sig) (#pht:(p:pht s{not_full p.repr}))
 ```pulse
 fn lookup (#s:pht_sig) (#pht:(p:pht s{not_full p.repr}))  
           (ht:ht s) (k:s.keyt)
-  requires models s pht ht
+  requires models s ht pht
   returns  o:(o:option s.valt{o == PHT.lookup pht k})
-  ensures  models s pht ht
+  ensures  models s ht pht
 {
   let o = pulse_lookup_index #s #pht ht k;
   match o {
@@ -118,149 +120,137 @@ fn lookup (#s:pht_sig) (#pht:(p:pht s{not_full p.repr}))
 ```pulse
 fn insert (#s:pht_sig) (#pht:(p:pht s{not_full p.repr})) 
           (ht:ht s) (k:s.keyt) (v:s.valt)
-  requires models s pht ht
-  ensures  models s (PHT.insert pht k v) ht
+  requires models s ht pht
+  ensures  models s ht (PHT.insert pht k v)
 {
   let sz = ht.sz;
-  let a = ht.contents;
-  let cidx = canonical_index k sz;
-  let mut off = coerce_nat 0;
+  let cidx = canonical_index_us k sz;
+  let mut off = 0sz;
   let mut cont = true;
 
-  unfold (models s pht ht);
+  unfold (models s ht pht);
 
-  while (let voff = !off; let vcont = !cont; (voff <= sz && vcont = true))
-  invariant b. exists (voff:nat) (vcont:bool). (
+  while (let voff = !off; let vcont = !cont; (voff <= sz && vcont = true)) 
+  invariant b. exists (voff:US.t) (vcont:bool). (
     R.pts_to off full_perm voff **
     R.pts_to cont full_perm vcont **
     `@(if vcont 
       then A.pts_to ht.contents full_perm pht.repr
       else A.pts_to ht.contents full_perm (PHT.insert pht k v).repr) **
     pure (
-      voff >= 0 /\ voff <= sz /\
-      strong_all_used_not_by pht.repr cidx voff k /\
-      walk pht.repr cidx k voff == lookup_repr pht.repr k /\
-      insert_repr_walk #s #sz #pht.spec pht.repr k v voff cidx () () == insert_repr #s #sz #pht.spec pht.repr k v /\
+      voff <= sz /\
+      strong_all_used_not_by pht.repr (US.v cidx) (US.v voff) k /\
+      walk pht.repr (US.v cidx) k (US.v voff) == lookup_repr pht.repr k /\
+      insert_repr_walk #s #pht.sz #pht.spec pht.repr k v (US.v voff) (US.v cidx) () () == insert_repr #s #pht.sz #pht.spec pht.repr k v /\
       b == (voff <= sz && vcont = true)
     ))
   {
     let voff = !off;
     if (voff = sz) {
-      // this case is not reachable, needs proof?
-      ()
+      cont := false;
+      assert_ (A.pts_to ht.contents full_perm pht.repr);
     } else {
-      let idx = (cidx+voff)%sz;
-      let c = op_Array_Index_nat ht.contents #full_perm #pht.repr idx;
+      let idx = modulo_us sz cidx voff;
+      let c = op_Array_Index ht.contents #full_perm #pht.repr idx;
       match c {
         Used k' v' -> { 
           if (k' = k) {
-            op_Array_Assignment_nat ht.contents idx (mk_used_cell k v);
+            op_Array_Assignment ht.contents idx (mk_used_cell k v);
             cont := false;
-            assert_ (pure (insert_repr #s #sz #pht.spec pht.repr k v `Seq.equal` 
-              Seq.upd pht.repr idx (mk_used_cell k v))); 
-            ()
+            assert_ (pure (insert_repr #s #pht.sz #pht.spec pht.repr k v `Seq.equal` 
+              Seq.upd pht.repr (US.v idx) (mk_used_cell k v))); 
           } else {
-            off := voff + 1;
-            ()
+            off := voff + 1sz;
           } 
         }
         Clean -> {
-          op_Array_Assignment_nat ht.contents idx (mk_used_cell k v);
+          op_Array_Assignment ht.contents idx (mk_used_cell k v);
           cont := false;
-          assert_ (pure (insert_repr #s #sz #pht.spec pht.repr k v `Seq.equal` 
-            Seq.upd pht.repr idx (mk_used_cell k v)));
-          ()
+          assert_ (pure (insert_repr #s #pht.sz #pht.spec pht.repr k v `Seq.equal` 
+            Seq.upd pht.repr (US.v idx) (mk_used_cell k v)));
         }
         Zombie -> {
-          fold (models s pht ht);
+          fold (models s ht pht);
           let o = pulse_lookup_index #s #pht ht k;
-          unfold (models s pht ht);
+          unfold (models s ht pht);
           match o {
             Some p -> {
-              op_Array_Assignment_nat ht.contents (snd p) Zombie;
-              op_Array_Assignment_nat ht.contents idx (mk_used_cell k v);
+              op_Array_Assignment ht.contents (snd p) Zombie;
+              op_Array_Assignment ht.contents idx (mk_used_cell k v);
               cont := false;
-              assert_ (pure (insert_repr #s #sz #pht.spec pht.repr k v `Seq.equal` 
-                Seq.upd (Seq.upd pht.repr (snd p) Zombie) idx (mk_used_cell k v)));
-              ()
+              assert_ (pure (insert_repr #s #pht.sz #pht.spec pht.repr k v `Seq.equal` 
+                Seq.upd (Seq.upd pht.repr (US.v (snd p)) Zombie) (US.v idx) (mk_used_cell k v)));
             }
             None -> { 
-              op_Array_Assignment_nat ht.contents idx (mk_used_cell k v); 
+              op_Array_Assignment ht.contents idx (mk_used_cell k v); 
               cont := false;
-              assert_ (pure (insert_repr #s #sz #pht.spec pht.repr k v `Seq.equal` Seq.upd pht.repr idx (mk_used_cell k v)));
-              ()
+              assert_ (pure (insert_repr #s #pht.sz #pht.spec pht.repr k v `Seq.equal` Seq.upd pht.repr (US.v idx) (mk_used_cell k v)));
             }
           };
         }
       };
     };
   };
-  fold (models s (PHT.insert pht k v) ht);
-  ()
+  fold (models s ht (PHT.insert pht k v));
 }
 ```
 
 ```pulse
 fn delete (#s:pht_sig) (#pht:pht s) 
           (ht:ht s) (k:s.keyt)
-  requires models s pht ht
-  ensures  models s (PHT.delete pht k) ht
+  requires models s ht pht
+  ensures  models s ht (PHT.delete pht k)
 {
   let sz = ht.sz;
-  let a = ht.contents;
-  let cidx = canonical_index k sz;
-  let mut off = coerce_nat 0;
+  let cidx = canonical_index_us k sz;
+  let mut off = 0sz;
   let mut cont = true;
 
-  unfold (models s pht ht);
+  unfold (models s ht pht);
 
   while (let voff = !off; let vcont = !cont; (voff <= sz && vcont = true))
-  invariant b. exists (voff:nat) (vcont:bool). (
+  invariant b. exists (voff:US.t) (vcont:bool). (
     R.pts_to off full_perm voff **
     R.pts_to cont full_perm vcont **
     `@(if vcont 
       then A.pts_to ht.contents full_perm pht.repr
       else A.pts_to ht.contents full_perm (PHT.delete pht k).repr) **
     pure (
-      voff >= 0 /\ voff <= sz /\
-      all_used_not_by pht.repr cidx voff k /\
-      walk pht.repr cidx k voff == lookup_repr pht.repr k /\
-      delete_repr_walk #s #sz #pht.spec pht.repr k voff cidx () () == delete_repr #s #sz #pht.spec pht.repr k /\
+      voff <= sz /\
+      all_used_not_by pht.repr (US.v cidx) (US.v voff) k /\
+      walk pht.repr (US.v cidx) k (US.v voff) == lookup_repr pht.repr k /\
+      delete_repr_walk #s #pht.sz #pht.spec pht.repr k (US.v voff) (US.v cidx) () () == delete_repr #s #pht.sz #pht.spec pht.repr k /\
       b == (voff <= sz && vcont = true)
     ))
   {
     let voff = !off;
-    if (voff=sz) {
-      ()
+    if (voff = sz) {
+      cont := false;
+      assert_ (A.pts_to ht.contents full_perm pht.repr);
     } else {
-      let idx = (cidx+voff)%sz;
-      let c = op_Array_Index_nat ht.contents #full_perm #pht.repr idx;
+      let idx = modulo_us sz cidx voff;
+      let c = op_Array_Index ht.contents #full_perm #pht.repr idx;
       match c {
         Used k' v' -> { 
           if (k' = k) {
-            op_Array_Assignment_nat ht.contents idx Zombie;
+            op_Array_Assignment ht.contents idx Zombie #pht.repr;
             cont := false;
-            assert_ (pure (pht.repr @@ idx == Used k v'));
-            assert_ (pure (Seq.upd pht.repr idx Zombie `Seq.equal` (PHT.delete pht k).repr));
-            ()
+            assert_ (pure (pht.repr @@ US.v idx == Used k v'));
+            assert_ (pure (Seq.upd pht.repr (US.v idx) Zombie `Seq.equal` (PHT.delete pht k).repr));
           } else {
-            off := voff + 1;
-            ()
+            off := voff + 1sz;
           } 
         }
         Clean -> {
           cont := false;
           assert_ (pure (pht.repr == (PHT.delete pht k).repr));
-          ()
         }
         Zombie -> { 
-          off := voff + 1;
-          () 
+          off := voff + 1sz;
         }
       };
     };
   };
-  fold (models s (PHT.delete pht k) ht);
-  ()
+  fold (models s ht (PHT.delete pht k));
 }
 ```
